\documentclass[11pt, a4paper]{article}\usepackage[]{graphicx}\usepackage[]{xcolor}
% maxwidth is the original width if it is less than linewidth
% otherwise use linewidth (to make sure the graphics do not exceed the margin)
\makeatletter
\def\maxwidth{ %
  \ifdim\Gin@nat@width>\linewidth
    \linewidth
  \else
    \Gin@nat@width
  \fi
}
\makeatother

\definecolor{fgcolor}{rgb}{0.345, 0.345, 0.345}
\newcommand{\hlnum}[1]{\textcolor[rgb]{0.686,0.059,0.569}{#1}}%
\newcommand{\hlsng}[1]{\textcolor[rgb]{0.192,0.494,0.8}{#1}}%
\newcommand{\hlcom}[1]{\textcolor[rgb]{0.678,0.584,0.686}{\textit{#1}}}%
\newcommand{\hlopt}[1]{\textcolor[rgb]{0,0,0}{#1}}%
\newcommand{\hldef}[1]{\textcolor[rgb]{0.345,0.345,0.345}{#1}}%
\newcommand{\hlkwa}[1]{\textcolor[rgb]{0.161,0.373,0.58}{\textbf{#1}}}%
\newcommand{\hlkwb}[1]{\textcolor[rgb]{0.69,0.353,0.396}{#1}}%
\newcommand{\hlkwc}[1]{\textcolor[rgb]{0.333,0.667,0.333}{#1}}%
\newcommand{\hlkwd}[1]{\textcolor[rgb]{0.737,0.353,0.396}{\textbf{#1}}}%
\let\hlipl\hlkwb

\usepackage{framed}
\makeatletter
\newenvironment{kframe}{%
 \def\at@end@of@kframe{}%
 \ifinner\ifhmode%
  \def\at@end@of@kframe{\end{minipage}}%
  \begin{minipage}{\columnwidth}%
 \fi\fi%
 \def\FrameCommand##1{\hskip\@totalleftmargin \hskip-\fboxsep
 \colorbox{shadecolor}{##1}\hskip-\fboxsep
     % There is no \\@totalrightmargin, so:
     \hskip-\linewidth \hskip-\@totalleftmargin \hskip\columnwidth}%
 \MakeFramed {\advance\hsize-\width
   \@totalleftmargin\z@ \linewidth\hsize
   \@setminipage}}%
 {\par\unskip\endMakeFramed%
 \at@end@of@kframe}
\makeatother

\definecolor{shadecolor}{rgb}{.97, .97, .97}
\definecolor{messagecolor}{rgb}{0, 0, 0}
\definecolor{warningcolor}{rgb}{1, 0, 1}
\definecolor{errorcolor}{rgb}{1, 0, 0}
\newenvironment{knitrout}{}{} % an empty environment to be redefined in TeX

\usepackage{alltt}

\usepackage[top = 1 in, bottom = 1 in, left = 1 in, right = 1 in ]{geometry}

\usepackage{amsmath, amssymb, amsfonts}
\usepackage{enumerate}
\usepackage{array}
\usepackage{multirow}
\usepackage{dingbat}
\usepackage{fontawesome5}
\usepackage{tasks}
\usepackage{bbding}
\usepackage{twemojis}
% how to use bull's eye ----- \scalebox{2.0}{\twemoji{bullseye}}
\usepackage{fontspec}
\usepackage{customdice}
% how to put dice face ------ \dice{2}

\title{MSMS 206 : Practical 06 - Supplementary Derivations}
\author{Ananda Biswas}
\date{\today}

\newfontface\myfont{Myfont1-Regular.ttf}[LetterSpace=0.05em]
% how to use ---- {\setlength{\spaceskip}{1em plus 0.5em minus 0.5em} \fontsize{17}{20}\myfont --write text here-- \par}

\newfontface\cbfont{CaveatBrush-Regular.ttf}
% how to use --- \myfont --write text here--
\IfFileExists{upquote.sty}{\usepackage{upquote}}{}
\begin{document}

\maketitle

\faArrowAltCircleRight[regular]

\[
f(t; \alpha, \lambda) = \frac{\alpha}{\lambda} \left( \frac{t}{\lambda} \right)^{\alpha - 1} e^{-(t/\lambda)^\alpha}, \quad t > 0.
\]


For a sample of size $n$, the likelihood function is given by

\begin{align*}
L(\alpha, \lambda) &= \prod \limits_{i = 1}^{n} \frac{\alpha}{\lambda} \left( \frac{x_i}{\lambda} \right)^{\alpha - 1} e^{-(x_i / \lambda)^\alpha} \\
&= \left( \dfrac{\alpha}{\lambda} \right)^n \left( \prod \limits_{i = 1}^{n}  \dfrac{x_i}{\lambda} \right)^{\alpha - 1} \text{exp}\left\{- \sum \limits_{i = 1}^{n} \left( \dfrac{x_i}{\lambda}\ \right)^{\alpha} \right\}.
\end{align*}

\vspace{0.5cm}

The log-likelihood function is given by

$$l(\alpha, \lambda) = n \log \alpha - n \log \lambda + (\alpha - 1) \sum_{i=1}^{n} \log \left( \frac{x_i}{\lambda} \right) - \sum_{i=1}^{n} \left( \frac{x_i}{\lambda} \right)^{\alpha}.$$

Now, 
\begin{align*}
\dfrac{\partial}{\partial \alpha} l(\alpha, \lambda) &= \dfrac{n}{\alpha} + \sum \limits_{i=1}^{n} \log \left( \dfrac{x_i}{\lambda} \right) - \sum \limits_{i=1}^{n} \left( \dfrac{x_i}{\lambda} \right)^{\alpha} \log \left( \dfrac{x_i}{\lambda} \right) = u(\alpha, \lambda) \text{, say}
\end{align*}

and

\begin{align*}
\dfrac{\partial}{\partial \lambda} l(\alpha, \lambda) &= -\dfrac{n}{\lambda} + (\alpha - 1) \sum \limits_{i=1}^{n} \dfrac{\lambda}{x_i} \cdot \left( -\dfrac{x_i}{\lambda^2} \right) + \sum \limits_{i=1}^{n} \dfrac{\alpha \cdot x_i^{\alpha}}{\lambda^{\alpha + 1}}\\[0.3cm]
&= -\dfrac{n}{\lambda} - (\alpha - 1) \dfrac{n}{\lambda} + \sum \limits_{i=1}^{n} \dfrac{\alpha \cdot x_i^{\alpha}}{\lambda^{\alpha + 1}}\\[0.3cm]
&= -\dfrac{n \alpha}{\lambda} + \sum \limits_{i=1}^{n} \dfrac{\alpha \cdot x_i^{\alpha}}{\lambda^{\alpha + 1}} = v(\alpha, \lambda) \text{, say}.
\end{align*}

\newpage

Now,
\begin{align*}
u_{\alpha}(\alpha, \lambda) &= \dfrac{\partial}{\partial \alpha} u(\alpha, \lambda) = -\dfrac{n}{\alpha^2} - \sum \limits_{i=1}^{n} \left( \dfrac{x_i}{\lambda} \right)^{\alpha} \left[ \log \left( \dfrac{x_i}{\lambda} \right) \right]^2;\\[0.3cm]
u_{\lambda}(\alpha, \lambda) &= \dfrac{\partial}{\partial \lambda} u(\alpha, \lambda) =
\sum \limits_{i=1}^{n} \dfrac{\lambda}{x_i} \cdot \left( -\dfrac{x_i}{\lambda^2} \right)
- \sum \limits_{i=1}^{n} \left[\dfrac{(-\alpha) x_i^{\alpha}}{\lambda^{\alpha + 1}} \log \left( \dfrac{x_i}{\lambda} \right) + \left( \dfrac{x_i}{\lambda} \right)^{\alpha}\dfrac{\lambda}{x_i} \cdot \left( -\dfrac{x_i}{\lambda^2} \right) \right]\\[0.3cm]
&\phantom{= \frac{\partial}{\partial \lambda} u(\alpha, \lambda) \hspace{0.1cm}} = -\dfrac{n}{\lambda} + \sum \limits_{i=1}^{n} \left[\dfrac{x_i^{\alpha}}{\lambda^{\alpha + 1}} \left( \alpha \log \left( \dfrac{x_i}{\lambda} \right) + 1 \right) \right].
\end{align*}

Also,
\begin{align*}
v_{\alpha}(\alpha, \lambda) &= \dfrac{\partial}{\partial \alpha} v(\alpha, \lambda) =
-\dfrac{n}{\lambda} + \sum \limits_{i=1}^{n} \left[\dfrac{x_i^{\alpha}}{\lambda^{\alpha + 1}}
+ \dfrac{\alpha}{\lambda} \left( \dfrac{x_i}{\lambda} \right)^{\alpha} \log \left( \dfrac{x_i}{\lambda} \right) \right]\\[0.3cm]
&\phantom{= \frac{\partial}{\partial \alpha} v(\alpha, \lambda) \hspace{0.1cm}} =
-\dfrac{n}{\lambda} + \sum \limits_{i=1}^{n} \left[\dfrac{x_i^{\alpha}}{\lambda^{\alpha + 1}}
\left( \alpha \log \left( \dfrac{x_i}{\lambda} \right) + 1 \right) \right];\\[0.3cm]
v_{\lambda}(\alpha, \lambda) &= \dfrac{\partial}{\partial \lambda} v(\alpha, \lambda) =
\dfrac{n \alpha}{\lambda^2} - \sum \limits_{i=1}^{n} \dfrac{\alpha(\alpha + 1) x_i^{\alpha}}{\lambda^{\alpha + 2}}.
\end{align*}


\end{document}
